src/FS.v
@@ -21,8 +21,15 @@ Require Import Array.
 Set Implicit Arguments.
 Import ListNotations.
 
-Definition compute_xparams (cache_blocks data_bitmaps inode_bitmaps : addr) cache_blocks_ok :
-  (MemLog.xparams * Inode.xparams * Balloc.xparams * Balloc.xparams * addr) :=
+Record xparams := {
+  FSXPMemLog : MemLog.xparams;
+  FSXPInode : Inode.xparams;
+  FSXPInodeAlloc : Balloc.xparams;
+  FSXPBlockAlloc : Balloc.xparams;
+  FSXPMaxBlock : addr
+}.
+
+Definition compute_xparams (cache_blocks data_bitmaps inode_bitmaps : addr) cache_blocks_ok :=
   let data_blocks := data_bitmaps ^* BALLOC.items_per_valu in
   let inode_blocks := inode_bitmaps ^* BALLOC.items_per_valu ^/ INODE.items_per_valu in
   let inode_base := data_blocks in
@@ -30,36 +37,37 @@ Definition compute_xparams (cache_blocks data_bitmaps inode_bitmaps : addr) cach
   let log_base := balloc_base ^+ data_bitmaps in
   let log_size := $ MEMLOG.addr_per_block in
   let max_addr := log_base ^+ $4 ^+ log_size in
-  (MemLog.Build_xparams (@Cache.Build_xparams cache_blocks cache_blocks_ok)
-                        log_base (log_base ^+ $1) (log_base ^+ $2) (log_base ^+ $3) log_size,
-   Inode.Build_xparams inode_base inode_blocks,
-   Balloc.Build_xparams (inode_base ^+ inode_blocks) inode_bitmaps,
-   Balloc.Build_xparams balloc_base data_bitmaps,
+  (Build_xparams
+   (MemLog.Build_xparams (@Cache.Build_xparams cache_blocks cache_blocks_ok)
+                         log_base (log_base ^+ $1) (log_base ^+ $2) (log_base ^+ $3) log_size)
+   (Inode.Build_xparams inode_base inode_blocks)
+   (Balloc.Build_xparams (inode_base ^+ inode_blocks) inode_bitmaps)
+   (Balloc.Build_xparams balloc_base data_bitmaps)
    max_addr).
 
-Definition file_len T lxp ixp inum mscs rx : prog T :=
-  mscs <- MEMLOG.begin lxp mscs;
-  let2 (mscs, len) <- BFILE.bflen lxp ixp inum mscs;
-  let2 (mscs, ok) <- MEMLOG.commit lxp mscs;
+Definition file_len T fsxp inum mscs rx : prog T :=
+  mscs <- MEMLOG.begin (FSXPMemLog fsxp) mscs;
+  let2 (mscs, len) <- BFILE.bflen (FSXPMemLog fsxp) (FSXPInode fsxp) inum mscs;
+  let2 (mscs, ok) <- MEMLOG.commit (FSXPMemLog fsxp) mscs;
   rx (mscs, len ^* $ (valulen / 8)).
 
-Definition read_block T lxp ixp inum off mscs rx : prog T :=
-  mscs <- MEMLOG.begin lxp mscs;
-  let2 (mscs, b) <- BFILE.bfread lxp ixp inum off mscs;
-  let2 (mscs, ok) <- MEMLOG.commit lxp mscs;
+Definition read_block T fsxp inum off mscs rx : prog T :=
+  mscs <- MEMLOG.begin (FSXPMemLog fsxp) mscs;
+  let2 (mscs, b) <- BFILE.bfread (FSXPMemLog fsxp) (FSXPInode fsxp) inum off mscs;
+  let2 (mscs, ok) <- MEMLOG.commit (FSXPMemLog fsxp) mscs;
   rx (mscs, b).
 
-Theorem read_block_ok : forall lxp bxp ixp inum off mscs,
+Theorem read_block_ok : forall fsxp inum off mscs,
   {< m F flist A f B v,
-  PRE    MEMLOG.rep lxp (NoTransaction m) mscs *
-         [[ (F * BFILE.rep bxp ixp flist)%pred (list2mem m) ]] *
+  PRE    MEMLOG.rep (FSXPMemLog fsxp) (NoTransaction m) mscs *
+         [[ (F * BFILE.rep (FSXPBlockAlloc fsxp) (FSXPInode fsxp) flist)%pred (list2mem m) ]] *
          [[ (A * #inum |-> f)%pred (list2nmem flist) ]] *
          [[ (B * #off |-> v)%pred (list2nmem (BFILE.BFData f)) ]]
   POST:(mscs',r)
-         MEMLOG.rep lxp (NoTransaction m) mscs' *
+         MEMLOG.rep (FSXPMemLog fsxp) (NoTransaction m) mscs' *
          [[ r = v ]]
-  CRASH  MEMLOG.log_intact lxp m
-  >} read_block lxp ixp inum off mscs.
+  CRASH  MEMLOG.log_intact (FSXPMemLog fsxp) m
+  >} read_block fsxp inum off mscs.
 Proof.
 (* XXX why doesn't this proof, which unfolds MEM.log_intact first, go through?
   unfold read_block, MEMLOG.log_intact.
@@ -75,21 +83,21 @@ Proof.
   unfold MEMLOG.log_intact; cancel.
 Qed.
 
-Theorem read_block_recover_ok : forall lxp bxp ixp inum off mscs,
+Theorem read_block_recover_ok : forall fsxp inum off mscs,
   {< m F flist A f B v,
-  PRE     MEMLOG.rep lxp (NoTransaction m) mscs *
-          [[ (F * BFILE.rep bxp ixp flist)%pred (list2mem m) ]] *
+  PRE     MEMLOG.rep (FSXPMemLog fsxp) (NoTransaction m) mscs *
+          [[ (F * BFILE.rep (FSXPBlockAlloc fsxp) (FSXPInode fsxp) flist)%pred (list2mem m) ]] *
           [[ (A * #inum |-> f)%pred (list2nmem flist) ]] *
           [[ (B * #off |-> v)%pred (list2nmem (BFILE.BFData f)) ]]
   POST:(mscs',r)
-          MEMLOG.rep lxp (NoTransaction m) mscs' *
+          MEMLOG.rep (FSXPMemLog fsxp) (NoTransaction m) mscs' *
           [[ r = v ]]
-  CRASH:mscs' MEMLOG.rep lxp (NoTransaction m) mscs'
-  >} read_block lxp ixp inum off mscs >> MEMLOG.recover lxp.
+  CRASH:mscs' MEMLOG.rep (FSXPMemLog fsxp) (NoTransaction m) mscs'
+  >} read_block fsxp inum off mscs >> MEMLOG.recover (FSXPMemLog fsxp).
 Proof.
   intros.
   unfold forall_helper; intros m F flist A f B v.
-  exists (MEMLOG.log_intact lxp m).
+  exists (MEMLOG.log_intact (FSXPMemLog fsxp) m).
 
   intros.
   eapply pimpl_ok3.
@@ -109,31 +117,31 @@ Proof.
   admit.
 Qed.
 
-Definition write_block_inbounds T lxp ixp inum off v mscs rx : prog T :=
-  mscs <- MEMLOG.begin lxp mscs;
-  mscs <- BFILE.bfwrite lxp ixp inum off v mscs;
-  let2 (mscs, ok) <- MEMLOG.commit lxp mscs;
+Definition write_block_inbounds T fsxp inum off v mscs rx : prog T :=
+  mscs <- MEMLOG.begin (FSXPMemLog fsxp) mscs;
+  mscs <- BFILE.bfwrite (FSXPMemLog fsxp) (FSXPInode fsxp) inum off v mscs;
+  let2 (mscs, ok) <- MEMLOG.commit (FSXPMemLog fsxp) mscs;
   rx (mscs, ok).
 
-Theorem write_block_inbounds_ok : forall lxp bxp ixp inum off v mscs,
+Theorem write_block_inbounds_ok : forall fsxp inum off v mscs,
   {< m F flist A f B v0,
-  PRE     MEMLOG.rep lxp (NoTransaction m) mscs *
-          [[ (F * BFILE.rep bxp ixp flist)%pred (list2mem m) ]] *
+  PRE     MEMLOG.rep (FSXPMemLog fsxp) (NoTransaction m) mscs *
+          [[ (F * BFILE.rep (FSXPBlockAlloc fsxp) (FSXPInode fsxp) flist)%pred (list2mem m) ]] *
           [[ (A * #inum |-> f)%pred (list2nmem flist) ]] *
           [[ (B * #off |-> v0)%pred (list2nmem (BFILE.BFData f)) ]]
   POST:(mscs',ok)
-          [[ ok = false ]] * MEMLOG.rep lxp (NoTransaction m) mscs' \/
+          [[ ok = false ]] * MEMLOG.rep (FSXPMemLog fsxp) (NoTransaction m) mscs' \/
           [[ ok = true ]] * exists m' flist' f',
-          MEMLOG.rep lxp (NoTransaction m') mscs' *
-          [[ (F * BFILE.rep bxp ixp flist')%pred (list2mem m') ]] *
+          MEMLOG.rep (FSXPMemLog fsxp) (NoTransaction m') mscs' *
+          [[ (F * BFILE.rep (FSXPBlockAlloc fsxp) (FSXPInode fsxp) flist')%pred (list2mem m') ]] *
           [[ (A * #inum |-> f')%pred (list2nmem flist') ]] *
           [[ (B * #off |-> v)%pred (list2nmem (BFILE.BFData f')) ]]
-  CRASH   MEMLOG.log_intact lxp m \/ exists m' flist' f',
-          MEMLOG.log_intact lxp m' *
-          [[ (F * BFILE.rep bxp ixp flist')%pred (list2mem m') ]] *
+  CRASH   MEMLOG.log_intact (FSXPMemLog fsxp) m \/ exists m' flist' f',
+          MEMLOG.log_intact (FSXPMemLog fsxp) m' *
+          [[ (F * BFILE.rep (FSXPBlockAlloc fsxp) (FSXPInode fsxp) flist')%pred (list2mem m') ]] *
           [[ (A * #inum |-> f')%pred (list2nmem flist') ]] *
           [[ (B * #off |-> v)%pred (list2nmem (BFILE.BFData f')) ]]
-  >} write_block_inbounds lxp ixp inum off v mscs.
+  >} write_block_inbounds fsxp inum off v mscs.
 Proof.
   unfold write_block_inbounds.
   hoare.
@@ -142,32 +150,32 @@ Proof.
   unfold MEMLOG.log_intact; cancel.
 Qed.
 
-Theorem write_block_inbounds_recover_ok : forall lxp bxp ixp inum off v mscs,
+Theorem write_block_inbounds_recover_ok : forall fsxp inum off v mscs,
   {< m F flist A f B v0,
-  PRE     MEMLOG.rep lxp (NoTransaction m) mscs *
-          [[ (F * BFILE.rep bxp ixp flist)%pred (list2mem m) ]] *
+  PRE     MEMLOG.rep (FSXPMemLog fsxp) (NoTransaction m) mscs *
+          [[ (F * BFILE.rep (FSXPBlockAlloc fsxp) (FSXPInode fsxp) flist)%pred (list2mem m) ]] *
           [[ (A * #inum |-> f)%pred (list2nmem flist) ]] *
           [[ (B * #off |-> v0)%pred (list2nmem (BFILE.BFData f)) ]]
   POST:(mscs',ok)
-          [[ ok = false ]] * MEMLOG.rep lxp (NoTransaction m) mscs' \/
+          [[ ok = false ]] * MEMLOG.rep (FSXPMemLog fsxp) (NoTransaction m) mscs' \/
           [[ ok = true ]] * exists m' flist' f',
-          MEMLOG.rep lxp (NoTransaction m') mscs' *
-          [[ (F * BFILE.rep bxp ixp flist')%pred (list2mem m') ]] *
+          MEMLOG.rep (FSXPMemLog fsxp) (NoTransaction m') mscs' *
+          [[ (F * BFILE.rep (FSXPBlockAlloc fsxp) (FSXPInode fsxp) flist')%pred (list2mem m') ]] *
           [[ (A * #inum |-> f')%pred (list2nmem flist') ]] *
           [[ (B * #off |-> v)%pred (list2nmem (BFILE.BFData f')) ]]
   CRASH:mscs'
-          MEMLOG.rep lxp (NoTransaction m) mscs' \/ exists m' flist' f',
-          MEMLOG.rep lxp (NoTransaction m') mscs' *
-          [[ (F * BFILE.rep bxp ixp flist')%pred (list2mem m') ]] *
+          MEMLOG.rep (FSXPMemLog fsxp) (NoTransaction m) mscs' \/ exists m' flist' f',
+          MEMLOG.rep (FSXPMemLog fsxp) (NoTransaction m') mscs' *
+          [[ (F * BFILE.rep (FSXPBlockAlloc fsxp) (FSXPInode fsxp) flist')%pred (list2mem m') ]] *
           [[ (A * #inum |-> f')%pred (list2nmem flist') ]] *
           [[ (B * #off |-> v)%pred (list2nmem (BFILE.BFData f')) ]]
-  >} write_block_inbounds lxp ixp inum off v mscs >> MEMLOG.recover lxp.
+  >} write_block_inbounds fsxp inum off v mscs >> MEMLOG.recover (FSXPMemLog fsxp).
 Proof.
   intros.
   unfold forall_helper; intros m F flist A f B v0.
-  exists (MEMLOG.log_intact lxp m \/ exists m' flist' f',
-          MEMLOG.log_intact lxp m' *
-          [[ (F * BFILE.rep bxp ixp flist')%pred (list2mem m') ]] *
+  exists (MEMLOG.log_intact (FSXPMemLog fsxp) m \/ exists m' flist' f',
+          MEMLOG.log_intact (FSXPMemLog fsxp) m' *
+          [[ (F * BFILE.rep (FSXPBlockAlloc fsxp) (FSXPInode fsxp) flist')%pred (list2mem m') ]] *
           [[ (A * #inum |-> f')%pred (list2nmem flist') ]] *
           [[ (B * #off |-> v)%pred (list2nmem (BFILE.BFData f')) ]])%pred.
 
@@ -216,8 +224,8 @@ Proof.
   admit.
 Qed.
 
-Definition set_size_helper T lxp bxp ixp inum size mscs rx : prog T :=
-  let2 (mscs, curlen) <- BFILE.bflen lxp ixp inum mscs;
+Definition set_size_helper T fsxp inum size mscs rx : prog T :=
+  let2 (mscs, curlen) <- BFILE.bflen (FSXPMemLog fsxp) (FSXPInode fsxp) inum mscs;
   If (wlt_dec curlen size) {
     mscs <- For n < (size ^- curlen)
       Loopvar mscs <- mscs
@@ -225,7 +233,7 @@ Definition set_size_helper T lxp bxp ixp inum size mscs rx : prog T :=
       Invariant emp
       OnCrash emp
       Begin
-        let2 (mscs, ok) <- BFILE.bfgrow lxp bxp ixp inum mscs;
+        let2 (mscs, ok) <- BFILE.bfgrow (FSXPMemLog fsxp) (FSXPBlockAlloc fsxp) (FSXPInode fsxp) inum mscs;
         If (bool_dec ok false) {
           rx (mscs, false)
         } else {
@@ -241,97 +249,97 @@ Definition set_size_helper T lxp bxp ixp inum size mscs rx : prog T :=
       Invariant emp
       OnCrash emp
       Begin
-        mscs <- BFILE.bfshrink lxp bxp ixp inum mscs;
+        mscs <- BFILE.bfshrink (FSXPMemLog fsxp) (FSXPBlockAlloc fsxp) (FSXPInode fsxp) inum mscs;
         lrx mscs
     Rof;
 
     rx (mscs, true)
   }.
 
-Theorem set_size_helper_ok : forall lxp bxp ixp inum size mscs,
+Theorem set_size_helper_ok : forall fsxp inum size mscs,
     {< F A mbase m flist f,
-    PRE      MEMLOG.rep lxp (ActiveTxn mbase m) mscs *
+    PRE      MEMLOG.rep (FSXPMemLog fsxp) (ActiveTxn mbase m) mscs *
              [[ # size <= INODE.blocks_per_inode ]] *
-             [[ (F * BFILE.rep bxp ixp flist)%pred (list2mem m) ]] *
+             [[ (F * BFILE.rep (FSXPBlockAlloc fsxp) (FSXPInode fsxp) flist)%pred (list2mem m) ]] *
              [[ (A * #inum |-> f)%pred (list2nmem flist) ]]
     POST:(mscs',r)
-             [[ r = false ]] * MEMLOG.log_intact lxp mbase \/
+             [[ r = false ]] * MEMLOG.log_intact (FSXPMemLog fsxp) mbase \/
              [[ r = true ]] * exists m' flist' f',
-             MEMLOG.rep lxp (ActiveTxn mbase m') mscs' *
-             [[ (F * BFILE.rep bxp ixp flist')%pred (list2mem m') ]] *
+             MEMLOG.rep (FSXPMemLog fsxp) (ActiveTxn mbase m') mscs' *
+             [[ (F * BFILE.rep (FSXPBlockAlloc fsxp) (FSXPInode fsxp) flist')%pred (list2mem m') ]] *
              [[ (A * #inum |-> f')%pred (list2nmem flist') ]] *
              [[ BFILE.BFData f' = (firstn #size (BFILE.BFData f)) ++
                                   (repeat $0 (#size - length (BFILE.BFData f))) ]]
-    CRASH    MEMLOG.log_intact lxp mbase
-    >} set_size_helper lxp bxp ixp inum size mscs.
+    CRASH    MEMLOG.log_intact (FSXPMemLog fsxp) mbase
+    >} set_size_helper fsxp inum size mscs.
 Proof.
   admit.
 Qed.
 
-Definition set_size T lxp bxp ixp inum size mscs rx : prog T :=
-  mscs <- MEMLOG.begin lxp mscs;
-  let2 (mscs, ok) <- set_size_helper lxp bxp ixp inum size mscs;
+Definition set_size T fsxp inum size mscs rx : prog T :=
+  mscs <- MEMLOG.begin (FSXPMemLog fsxp) mscs;
+  let2 (mscs, ok) <- set_size_helper fsxp inum size mscs;
   If (bool_dec ok true) {
-    let2 (mscs, ok) <- MEMLOG.commit lxp mscs;
+    let2 (mscs, ok) <- MEMLOG.commit (FSXPMemLog fsxp) mscs;
     rx (mscs, ok)
   } else {
-    mscs <- MEMLOG.abort lxp mscs;
+    mscs <- MEMLOG.abort (FSXPMemLog fsxp) mscs;
     rx (mscs, false)
   }.
 
-Definition write_block T lxp bxp ixp inum off v mscs rx : prog T :=
-  mscs <- MEMLOG.begin lxp mscs;
-  let2 (mscs, curlen) <- BFILE.bflen lxp ixp inum mscs;
+Definition write_block T fsxp inum off v mscs rx : prog T :=
+  mscs <- MEMLOG.begin (FSXPMemLog fsxp) mscs;
+  let2 (mscs, curlen) <- BFILE.bflen (FSXPMemLog fsxp) (FSXPInode fsxp) inum mscs;
   If (wlt_dec off curlen) {
-    mscs <- BFILE.bfwrite lxp ixp inum off v mscs;
-    let2 (mscs, ok) <- MEMLOG.commit lxp mscs;
+    mscs <- BFILE.bfwrite (FSXPMemLog fsxp) (FSXPInode fsxp) inum off v mscs;
+    let2 (mscs, ok) <- MEMLOG.commit (FSXPMemLog fsxp) mscs;
     rx (mscs, ok)
   } else {
-    let2 (mscs, ok) <- set_size_helper lxp bxp ixp inum (off ^+ $1) mscs;
+    let2 (mscs, ok) <- set_size_helper fsxp inum (off ^+ $1) mscs;
     If (bool_dec ok false) {
-      mscs <- MEMLOG.abort lxp mscs;
+      mscs <- MEMLOG.abort (FSXPMemLog fsxp) mscs;
       rx (mscs, false)
     } else {
-      mscs <- BFILE.bfwrite lxp ixp inum off v mscs;
-      let2 (mscs, ok) <- MEMLOG.commit lxp mscs;
+      mscs <- BFILE.bfwrite (FSXPMemLog fsxp) (FSXPInode fsxp) inum off v mscs;
+      let2 (mscs, ok) <- MEMLOG.commit (FSXPMemLog fsxp) mscs;
       rx (mscs, ok)
     }
   }.
 
-Definition readdir T lxp bxp ixp dnum mscs rx : prog T :=
-  mscs <- MEMLOG.begin lxp mscs;
-  let2 (mscs, files) <- SDIR.dslist lxp bxp ixp dnum mscs;
-  let2 (mscs, ok) <- MEMLOG.commit lxp mscs;
+Definition readdir T fsxp dnum mscs rx : prog T :=
+  mscs <- MEMLOG.begin (FSXPMemLog fsxp) mscs;
+  let2 (mscs, files) <- SDIR.dslist (FSXPMemLog fsxp) (FSXPBlockAlloc fsxp) (FSXPInode fsxp) dnum mscs;
+  let2 (mscs, ok) <- MEMLOG.commit (FSXPMemLog fsxp) mscs;
   rx (mscs, files).
 
-Definition create T lxp ibxp dbxp ixp dnum name mscs rx : prog T :=
-  mscs <- MEMLOG.begin lxp mscs;
-  let2 (mscs, oi) <- DIRALLOC.dacreate lxp ibxp dbxp ixp dnum name mscs;
+Definition create T fsxp dnum name mscs rx : prog T :=
+  mscs <- MEMLOG.begin (FSXPMemLog fsxp) mscs;
+  let2 (mscs, oi) <- DIRALLOC.dacreate (FSXPMemLog fsxp) (FSXPBlockAlloc fsxp) (FSXPInodeAlloc fsxp) (FSXPInode fsxp) dnum name mscs;
   match oi with
   | None =>
-    mscs <- MEMLOG.abort lxp mscs;
+    mscs <- MEMLOG.abort (FSXPMemLog fsxp) mscs;
     rx (mscs, None)
   | Some inum =>
-    let2 (mscs, ok) <- MEMLOG.commit lxp mscs;
+    let2 (mscs, ok) <- MEMLOG.commit (FSXPMemLog fsxp) mscs;
     match ok with
     | true => rx (mscs, Some inum)
     | false => rx (mscs, None)
     end
   end.
 
-Definition delete T lxp ibxp dbxp ixp dnum name mscs rx : prog T :=
-  mscs <- MEMLOG.begin lxp mscs;
-  let2 (mscs, ok) <- DIRALLOC.dadelete lxp ibxp dbxp ixp dnum name mscs;
+Definition delete T fsxp dnum name mscs rx : prog T :=
+  mscs <- MEMLOG.begin (FSXPMemLog fsxp) mscs;
+  let2 (mscs, ok) <- DIRALLOC.dadelete (FSXPMemLog fsxp) (FSXPBlockAlloc fsxp) (FSXPInodeAlloc fsxp) (FSXPInode fsxp) dnum name mscs;
   If (bool_dec ok true) {
-    let2 (mscs, ok) <- MEMLOG.commit lxp mscs;
+    let2 (mscs, ok) <- MEMLOG.commit (FSXPMemLog fsxp) mscs;
     rx (mscs, ok)
   } else {
-    mscs <- MEMLOG.abort lxp mscs;
+    mscs <- MEMLOG.abort (FSXPMemLog fsxp) mscs;
     rx (mscs, false)
   }.
 
-Definition lookup T lxp bxp ixp dnum name mscs rx : prog T :=
-  mscs <- MEMLOG.begin lxp mscs;
-  let2 (mscs, r) <- SDIR.dslookup lxp bxp ixp dnum name mscs;
-  let2 (mscs, ok) <- MEMLOG.commit lxp mscs;
+Definition lookup T fsxp dnum name mscs rx : prog T :=
+  mscs <- MEMLOG.begin (FSXPMemLog fsxp) mscs;
+  let2 (mscs, r) <- SDIR.dslookup (FSXPMemLog fsxp) (FSXPBlockAlloc fsxp) (FSXPInode fsxp) dnum name mscs;
+  let2 (mscs, ok) <- MEMLOG.commit (FSXPMemLog fsxp) mscs;
   rx (mscs, r).
